Completed Tail Call Optimization

06TreeCode/TreeCode.thy
@@ -16,6 +16,31 @@ type_synonym tree_stack_frame = "tclosure list \<times> tree_code list"
 
 datatype tree_code_state = TS "tclosure list" "tree_stack_frame list"
 
+fun full_block :: "tree_code list \<Rightarrow> nat \<rightharpoonup> nat" where
+  "full_block [] n = Some n"
+| "full_block (TLookup x # cd) n = full_block cd (Suc n)"
+| "full_block (TPushCon k # cd) n = full_block cd (Suc n)"
+| "full_block (TPushLam cd' d # cd) n = full_block cd (Suc n)"
+| "full_block (TApply # cd) 0 = None"
+| "full_block (TApply # cd) (Suc n) = full_block cd n"
+
+primrec full_code_closure :: "tree_code \<Rightarrow> bool" where
+  "full_code_closure (TLookup x) = True"
+| "full_code_closure (TPushCon k) = True"
+| "full_code_closure (TPushLam cd d) = (full_block cd 0 = Some 1 \<and> list_all full_code_closure cd)"
+| "full_code_closure TApply = True"
+
+primrec full_closure :: "tclosure \<Rightarrow> bool" where
+  "full_closure (TConst k) = True"
+| "full_closure (TLam env cd) = 
+    (list_all full_closure env \<and> full_block cd 0 = Some 1 \<and> list_all full_code_closure cd)"
+
+primrec full_frame :: "tree_stack_frame \<Rightarrow> bool" where
+  "full_frame (env, cd) = (list_all full_closure env \<and> list_all full_code_closure cd)"
+
+primrec full_state :: "tree_code_state \<Rightarrow> bool" where
+  "full_state (TS env s) = (list_all full_closure env \<and> list_all full_frame s)"
+
 inductive evalt :: "tree_code_state \<Rightarrow> tree_code_state \<Rightarrow> bool" (infix "\<leadsto>\<^sub>t" 50) where
   evt_lookup [simp]: "lookup env x = Some v \<Longrightarrow> 
     TS vs ((env, TLookup x # cd) # sfs) \<leadsto>\<^sub>t TS (v # vs) ((env, cd) # sfs)"
@@ -25,6 +50,19 @@ inductive evalt :: "tree_code_state \<Rightarrow> tree_code_state \<Rightarrow> 
 | evt_apply [simp]: "TS (v # TLam env' cd' # vs) ((env, TApply # cd) # sfs) \<leadsto>\<^sub>t 
     TS vs ((v # env', cd') # (env, cd) # sfs)"
 | evt_return [simp]: "TS vs ((env, []) # sfs) \<leadsto>\<^sub>t TS vs sfs"
+
+lemma [simp]: "full_block cd1 n = Some m \<Longrightarrow> full_block cd2 m = Some k \<Longrightarrow> 
+    full_block (cd1 @ cd2) n = Some k"
+  by (induction cd1 n rule: full_block.induct) simp_all
+
+lemma [simp]: "full_block cd 0 = Some (Suc 0) \<Longrightarrow> cd \<noteq> [] \<and> cd \<noteq> [TApply]"
+proof (induction cd)
+  case (Cons op cd)
+  thus ?case by (induction op) simp_all
+qed simp_all
+  
+lemma preservation [simp]: "\<Sigma> \<leadsto>\<^sub>t \<Sigma>' \<Longrightarrow> full_state \<Sigma> \<Longrightarrow> full_state \<Sigma>'"
+  by (induction \<Sigma> \<Sigma>' rule: evalt.induct) auto
 
 theorem determinismt: "\<Sigma> \<leadsto>\<^sub>t \<Sigma>' \<Longrightarrow> \<Sigma> \<leadsto>\<^sub>t \<Sigma>'' \<Longrightarrow> \<Sigma>' = \<Sigma>''"
 proof (induction \<Sigma> \<Sigma>' rule: evalt.induct)
